pulse/src/ocaml/plugin/generated/Pulse_Checker_Abs.ml
@@ -63,7 +63,7 @@ let rec (arrow_of_abs :
         (FStar_Sealed.seal
            (Obj.magic
               (FStar_Range.mk_range "Pulse.Checker.Abs.fst"
-                 (Prims.of_int (38)) (Prims.of_int (3)) (Prims.of_int (93))
+                 (Prims.of_int (38)) (Prims.of_int (3)) (Prims.of_int (89))
                  (Prims.of_int (5)))))
         (FStar_Tactics_Effect.lift_div_tac
            (fun uu___ -> t.Pulse_Syntax_Base.term1))
@@ -86,7 +86,7 @@ let rec (arrow_of_abs :
                           (Obj.magic
                              (FStar_Range.mk_range "Pulse.Checker.Abs.fst"
                                 (Prims.of_int (39)) (Prims.of_int (24))
-                                (Prims.of_int (93)) (Prims.of_int (5)))))
+                                (Prims.of_int (89)) (Prims.of_int (5)))))
                        (FStar_Tactics_Effect.lift_div_tac
                           (fun uu___1 -> Pulse_Typing_Env.fresh env))
                        (fun uu___1 ->
@@ -107,7 +107,7 @@ let rec (arrow_of_abs :
                                            "Pulse.Checker.Abs.fst"
                                            (Prims.of_int (40))
                                            (Prims.of_int (34))
-                                           (Prims.of_int (93))
+                                           (Prims.of_int (89))
                                            (Prims.of_int (5)))))
                                   (FStar_Tactics_Effect.lift_div_tac
                                      (fun uu___1 ->
@@ -131,7 +131,7 @@ let rec (arrow_of_abs :
                                                       "Pulse.Checker.Abs.fst"
                                                       (Prims.of_int (41))
                                                       (Prims.of_int (56))
-                                                      (Prims.of_int (93))
+                                                      (Prims.of_int (89))
                                                       (Prims.of_int (5)))))
                                              (FStar_Tactics_Effect.lift_div_tac
                                                 (fun uu___1 ->
@@ -158,7 +158,7 @@ let rec (arrow_of_abs :
                                                                  "Pulse.Checker.Abs.fst"
                                                                  (Prims.of_int (42))
                                                                  (Prims.of_int (41))
-                                                                 (Prims.of_int (93))
+                                                                 (Prims.of_int (89))
                                                                  (Prims.of_int (5)))))
                                                         (FStar_Tactics_Effect.lift_div_tac
                                                            (fun uu___1 ->
@@ -173,61 +173,22 @@ let rec (arrow_of_abs :
                                                                     (FStar_Range.mk_range
                                                                     "Pulse.Checker.Abs.fst"
                                                                     (Prims.of_int (43))
-                                                                    (Prims.of_int (30))
-                                                                    (Prims.of_int (45))
-                                                                    (Prims.of_int (29)))))
+                                                                    (Prims.of_int (16))
+                                                                    (Prims.of_int (43))
+                                                                    (Prims.of_int (36)))))
                                                                    (FStar_Sealed.seal
                                                                     (Obj.magic
                                                                     (FStar_Range.mk_range
                                                                     "Pulse.Checker.Abs.fst"
-                                                                    (Prims.of_int (46))
-                                                                    (Prims.of_int (6))
-                                                                    (Prims.of_int (93))
+                                                                    (Prims.of_int (44))
+                                                                    (Prims.of_int (4))
+                                                                    (Prims.of_int (89))
                                                                     (Prims.of_int (5)))))
                                                                    (FStar_Tactics_Effect.lift_div_tac
                                                                     (fun
                                                                     uu___1 ->
-                                                                    fun
-                                                                    uu___2 ->
-                                                                    match uu___2
-                                                                    with
-                                                                    | 
-                                                                    FStar_Pervasives_Native.None
-                                                                    ->
-                                                                    FStar_Pervasives_Native.None
-                                                                    | 
-                                                                    FStar_Pervasives_Native.Some
-                                                                    a ->
-                                                                    a.Pulse_Syntax_Base.annotated))
+                                                                    ascription.Pulse_Syntax_Base.annotated))
                                                                    (fun
-                                                                    uu___1 ->
-                                                                    (fun
-                                                                    annot_of_ascription
-                                                                    ->
-                                                                    Obj.magic
-                                                                    (FStar_Tactics_Effect.tac_bind
-                                                                    (FStar_Sealed.seal
-                                                                    (Obj.magic
-                                                                    (FStar_Range.mk_range
-                                                                    "Pulse.Checker.Abs.fst"
-                                                                    (Prims.of_int (47))
-                                                                    (Prims.of_int (16))
-                                                                    (Prims.of_int (47))
-                                                                    (Prims.of_int (46)))))
-                                                                    (FStar_Sealed.seal
-                                                                    (Obj.magic
-                                                                    (FStar_Range.mk_range
-                                                                    "Pulse.Checker.Abs.fst"
-                                                                    (Prims.of_int (48))
-                                                                    (Prims.of_int (4))
-                                                                    (Prims.of_int (93))
-                                                                    (Prims.of_int (5)))))
-                                                                    (FStar_Tactics_Effect.lift_div_tac
-                                                                    (fun
-                                                                    uu___1 ->
-                                                                    annot_of_ascription
-                                                                    ascription))
-                                                                    (fun
                                                                     uu___1 ->
                                                                     (fun
                                                                     annot ->
@@ -247,17 +208,17 @@ let rec (arrow_of_abs :
                                                                     (Obj.magic
                                                                     (FStar_Range.mk_range
                                                                     "Pulse.Checker.Abs.fst"
-                                                                    (Prims.of_int (53))
+                                                                    (Prims.of_int (49))
                                                                     (Prims.of_int (18))
-                                                                    (Prims.of_int (53))
+                                                                    (Prims.of_int (49))
                                                                     (Prims.of_int (39)))))
                                                                     (FStar_Sealed.seal
                                                                     (Obj.magic
                                                                     (FStar_Range.mk_range
                                                                     "Pulse.Checker.Abs.fst"
-                                                                    (Prims.of_int (55))
+                                                                    (Prims.of_int (51))
                                                                     (Prims.of_int (10))
-                                                                    (Prims.of_int (55))
+                                                                    (Prims.of_int (51))
                                                                     (Prims.of_int (91)))))
                                                                     (Obj.magic
                                                                     (arrow_of_abs
@@ -291,17 +252,17 @@ let rec (arrow_of_abs :
                                                                     (Obj.magic
                                                                     (FStar_Range.mk_range
                                                                     "Pulse.Checker.Abs.fst"
-                                                                    (Prims.of_int (58))
+                                                                    (Prims.of_int (54))
                                                                     (Prims.of_int (16))
-                                                                    (Prims.of_int (58))
+                                                                    (Prims.of_int (54))
                                                                     (Prims.of_int (52)))))
                                                                     (FStar_Sealed.seal
                                                                     (Obj.magic
                                                                     (FStar_Range.mk_range
                                                                     "Pulse.Checker.Abs.fst"
-                                                                    (Prims.of_int (59))
+                                                                    (Prims.of_int (55))
                                                                     (Prims.of_int (8))
-                                                                    (Prims.of_int (82))
+                                                                    (Prims.of_int (78))
                                                                     (Prims.of_int (37)))))
                                                                     (FStar_Tactics_Effect.lift_div_tac
                                                                     (fun
@@ -325,17 +286,17 @@ let rec (arrow_of_abs :
                                                                     (Obj.magic
                                                                     (FStar_Range.mk_range
                                                                     "Pulse.Checker.Abs.fst"
-                                                                    (Prims.of_int (61))
+                                                                    (Prims.of_int (57))
                                                                     (Prims.of_int (24))
-                                                                    (Prims.of_int (61))
+                                                                    (Prims.of_int (57))
                                                                     (Prims.of_int (69)))))
                                                                     (FStar_Sealed.seal
                                                                     (Obj.magic
                                                                     (FStar_Range.mk_range
                                                                     "Pulse.Checker.Abs.fst"
-                                                                    (Prims.of_int (65))
+                                                                    (Prims.of_int (61))
                                                                     (Prims.of_int (10))
-                                                                    (Prims.of_int (74))
+                                                                    (Prims.of_int (70))
                                                                     (Prims.of_int (93)))))
                                                                     (FStar_Tactics_Effect.lift_div_tac
                                                                     (fun
@@ -364,17 +325,17 @@ let rec (arrow_of_abs :
                                                                     (Obj.magic
                                                                     (FStar_Range.mk_range
                                                                     "Pulse.Checker.Abs.fst"
-                                                                    (Prims.of_int (70))
+                                                                    (Prims.of_int (66))
                                                                     (Prims.of_int (14))
-                                                                    (Prims.of_int (71))
+                                                                    (Prims.of_int (67))
                                                                     (Prims.of_int (45)))))
                                                                     (FStar_Sealed.seal
                                                                     (Obj.magic
                                                                     (FStar_Range.mk_range
                                                                     "Pulse.Checker.Abs.fst"
-                                                                    (Prims.of_int (67))
+                                                                    (Prims.of_int (63))
                                                                     (Prims.of_int (12))
-                                                                    (Prims.of_int (71))
+                                                                    (Prims.of_int (67))
                                                                     (Prims.of_int (45)))))
                                                                     (Obj.magic
                                                                     (FStar_Tactics_Effect.tac_bind
@@ -382,9 +343,9 @@ let rec (arrow_of_abs :
                                                                     (Obj.magic
                                                                     (FStar_Range.mk_range
                                                                     "Pulse.Checker.Abs.fst"
-                                                                    (Prims.of_int (71))
+                                                                    (Prims.of_int (67))
                                                                     (Prims.of_int (18))
-                                                                    (Prims.of_int (71))
+                                                                    (Prims.of_int (67))
                                                                     (Prims.of_int (44)))))
                                                                     (FStar_Sealed.seal
                                                                     (Obj.magic
@@ -449,17 +410,17 @@ let rec (arrow_of_abs :
                                                                     (Obj.magic
                                                                     (FStar_Range.mk_range
                                                                     "Pulse.Checker.Abs.fst"
-                                                                    (Prims.of_int (81))
+                                                                    (Prims.of_int (77))
                                                                     (Prims.of_int (12))
-                                                                    (Prims.of_int (82))
+                                                                    (Prims.of_int (78))
                                                                     (Prims.of_int (37)))))
                                                                     (FStar_Sealed.seal
                                                                     (Obj.magic
                                                                     (FStar_Range.mk_range
                                                                     "Pulse.Checker.Abs.fst"
-                                                                    (Prims.of_int (78))
+                                                                    (Prims.of_int (74))
                                                                     (Prims.of_int (10))
-                                                                    (Prims.of_int (82))
+                                                                    (Prims.of_int (78))
                                                                     (Prims.of_int (37)))))
                                                                     (Obj.magic
                                                                     (FStar_Tactics_Effect.tac_bind
@@ -467,9 +428,9 @@ let rec (arrow_of_abs :
                                                                     (Obj.magic
                                                                     (FStar_Range.mk_range
                                                                     "Pulse.Checker.Abs.fst"
-                                                                    (Prims.of_int (82))
+                                                                    (Prims.of_int (78))
                                                                     (Prims.of_int (16))
-                                                                    (Prims.of_int (82))
+                                                                    (Prims.of_int (78))
                                                                     (Prims.of_int (36)))))
                                                                     (FStar_Sealed.seal
                                                                     (Obj.magic
@@ -537,9 +498,51 @@ let rec (arrow_of_abs :
                                                                     c))
                                                                     })))))
                                                                     uu___1)))
-                                                                    uu___1)))
                                                              uu___1))) uu___1)))
                                        uu___1))) uu___1))) uu___)
+let (qualifier_compat :
+  Pulse_Typing_Env.env ->
+    Pulse_Syntax_Base.range ->
+      Pulse_Syntax_Base.qualifier FStar_Pervasives_Native.option ->
+        FStar_Reflection_V2_Data.aqualv ->
+          (unit, unit) FStar_Tactics_Effect.tac_repr)
+  =
+  fun uu___3 ->
+    fun uu___2 ->
+      fun uu___1 ->
+        fun uu___ ->
+          (fun g ->
+             fun r ->
+               fun q ->
+                 fun q' ->
+                   match (q, q') with
+                   | (FStar_Pervasives_Native.None,
+                      FStar_Reflection_V2_Data.Q_Explicit) ->
+                       Obj.magic
+                         (Obj.repr
+                            (FStar_Tactics_Effect.lift_div_tac
+                               (fun uu___ -> ())))
+                   | (FStar_Pervasives_Native.Some
+                      (Pulse_Syntax_Base.Implicit),
+                      FStar_Reflection_V2_Data.Q_Implicit) ->
+                       Obj.magic
+                         (Obj.repr
+                            (FStar_Tactics_Effect.lift_div_tac
+                               (fun uu___ -> ())))
+                   | (FStar_Pervasives_Native.Some
+                      (Pulse_Syntax_Base.Implicit),
+                      FStar_Reflection_V2_Data.Q_Meta uu___) ->
+                       Obj.magic
+                         (Obj.repr
+                            (FStar_Tactics_Effect.lift_div_tac
+                               (fun uu___1 -> ())))
+                   | uu___ ->
+                       Obj.magic
+                         (Obj.repr
+                            (Pulse_Typing_Env.fail g
+                               (FStar_Pervasives_Native.Some r)
+                               "Unexpected binder qualifier"))) uu___3 uu___2
+            uu___1 uu___
 let rec (rebuild_abs :
   Pulse_Typing_Env.env ->
     Pulse_Syntax_Base.st_term ->
@@ -553,13 +556,13 @@ let rec (rebuild_abs :
           (FStar_Sealed.seal
              (Obj.magic
                 (FStar_Range.mk_range "Pulse.Checker.Abs.fst"
-                   (Prims.of_int (98)) (Prims.of_int (4))
-                   (Prims.of_int (100)) (Prims.of_int (41)))))
+                   (Prims.of_int (101)) (Prims.of_int (4))
+                   (Prims.of_int (103)) (Prims.of_int (41)))))
           (FStar_Sealed.seal
              (Obj.magic
                 (FStar_Range.mk_range "Pulse.Checker.Abs.fst"
-                   (Prims.of_int (101)) (Prims.of_int (4))
-                   (Prims.of_int (154)) (Prims.of_int (47)))))
+                   (Prims.of_int (104)) (Prims.of_int (4))
+                   (Prims.of_int (160)) (Prims.of_int (47)))))
           (Obj.magic
              (debug_abs g
                 (fun uu___ ->
@@ -567,13 +570,13 @@ let rec (rebuild_abs :
                      (FStar_Sealed.seal
                         (Obj.magic
                            (FStar_Range.mk_range "Pulse.Checker.Abs.fst"
-                              (Prims.of_int (100)) (Prims.of_int (16))
-                              (Prims.of_int (100)) (Prims.of_int (40)))))
+                              (Prims.of_int (103)) (Prims.of_int (16))
+                              (Prims.of_int (103)) (Prims.of_int (40)))))
                      (FStar_Sealed.seal
                         (Obj.magic
                            (FStar_Range.mk_range "Pulse.Checker.Abs.fst"
-                              (Prims.of_int (98)) (Prims.of_int (26))
-                              (Prims.of_int (100)) (Prims.of_int (40)))))
+                              (Prims.of_int (101)) (Prims.of_int (26))
+                              (Prims.of_int (103)) (Prims.of_int (40)))))
                      (Obj.magic
                         (FStar_Tactics_V2_Builtins.term_to_string annot))
                      (fun uu___1 ->
@@ -584,17 +587,17 @@ let rec (rebuild_abs :
                                    (Obj.magic
                                       (FStar_Range.mk_range
                                          "Pulse.Checker.Abs.fst"
-                                         (Prims.of_int (98))
+                                         (Prims.of_int (101))
                                          (Prims.of_int (26))
-                                         (Prims.of_int (100))
+                                         (Prims.of_int (103))
                                          (Prims.of_int (40)))))
                                 (FStar_Sealed.seal
                                    (Obj.magic
                                       (FStar_Range.mk_range
                                          "Pulse.Checker.Abs.fst"
-                                         (Prims.of_int (98))
+                                         (Prims.of_int (101))
                                          (Prims.of_int (26))
-                                         (Prims.of_int (100))
+                                         (Prims.of_int (103))
                                          (Prims.of_int (40)))))
                                 (Obj.magic
                                    (FStar_Tactics_Effect.tac_bind
@@ -602,9 +605,9 @@ let rec (rebuild_abs :
                                          (Obj.magic
                                             (FStar_Range.mk_range
                                                "Pulse.Checker.Abs.fst"
-                                               (Prims.of_int (99))
+                                               (Prims.of_int (102))
                                                (Prims.of_int (16))
-                                               (Prims.of_int (99))
+                                               (Prims.of_int (102))
                                                (Prims.of_int (39)))))
                                       (FStar_Sealed.seal
                                          (Obj.magic
@@ -645,102 +648,153 @@ let rec (rebuild_abs :
                          (FStar_Sealed.seal
                             (Obj.magic
                                (FStar_Range.mk_range "Pulse.Checker.Abs.fst"
-                                  (Prims.of_int (103)) (Prims.of_int (15))
-                                  (Prims.of_int (103)) (Prims.of_int (53)))))
+                                  (Prims.of_int (106)) (Prims.of_int (15))
+                                  (Prims.of_int (106)) (Prims.of_int (34)))))
                          (FStar_Sealed.seal
                             (Obj.magic
                                (FStar_Range.mk_range "Pulse.Checker.Abs.fst"
-                                  (Prims.of_int (103)) (Prims.of_int (56))
-                                  (Prims.of_int (128)) (Prims.of_int (41)))))
+                                  (Prims.of_int (107)) (Prims.of_int (6))
+                                  (Prims.of_int (134)) (Prims.of_int (41)))))
                          (FStar_Tactics_Effect.lift_div_tac
                             (fun uu___1 ->
-                               Pulse_Readback.readback_ty
-                                 (FStar_Reflection_V2_Builtins.inspect_binder
-                                    b').FStar_Reflection_V2_Data.sort2))
+                               FStar_Reflection_V2_Builtins.inspect_binder b'))
                          (fun uu___1 ->
-                            (fun ty ->
+                            (fun b'1 ->
                                Obj.magic
                                  (FStar_Tactics_Effect.tac_bind
                                     (FStar_Sealed.seal
                                        (Obj.magic
                                           (FStar_Range.mk_range
                                              "Pulse.Checker.Abs.fst"
-                                             (Prims.of_int (104))
-                                             (Prims.of_int (17))
-                                             (Prims.of_int (104))
-                                             (Prims.of_int (34)))))
+                                             (Prims.of_int (107))
+                                             (Prims.of_int (6))
+                                             (Prims.of_int (107))
+                                             (Prims.of_int (56)))))
                                     (FStar_Sealed.seal
                                        (Obj.magic
                                           (FStar_Range.mk_range
                                              "Pulse.Checker.Abs.fst"
-                                             (Prims.of_int (105))
-                                             (Prims.of_int (6))
-                                             (Prims.of_int (128))
+                                             (Prims.of_int (107))
+                                             (Prims.of_int (57))
+                                             (Prims.of_int (134))
                                              (Prims.of_int (41)))))
-                                    (FStar_Tactics_Effect.lift_div_tac
-                                       (fun uu___1 ->
-                                          FStar_Reflection_V2_Builtins.inspect_comp
-                                            c'))
+                                    (Obj.magic
+                                       (qualifier_compat g
+                                          (b.Pulse_Syntax_Base.binder_ppname).Pulse_Syntax_Base.range
+                                          q b'1.FStar_Reflection_V2_Data.qual))
                                     (fun uu___1 ->
-                                       (fun comp ->
-                                          match (ty, comp) with
-                                          | (FStar_Pervasives_Native.Some
-                                             ty1,
-                                             FStar_Reflection_V2_Data.C_Total
-                                             res_ty) ->
-                                              Obj.magic
-                                                (Obj.repr
-                                                   (if
-                                                      Pulse_Syntax_Base.uu___is_Tm_Abs
-                                                        body.Pulse_Syntax_Base.term1
-                                                    then
-                                                      Obj.repr
-                                                        (FStar_Tactics_Effect.tac_bind
-                                                           (FStar_Sealed.seal
-                                                              (Obj.magic
-                                                                 (FStar_Range.mk_range
-                                                                    "Pulse.Checker.Abs.fst"
-                                                                    (Prims.of_int (109))
-                                                                    (Prims.of_int (20))
-                                                                    (Prims.of_int (109))
-                                                                    (Prims.of_int (68)))))
-                                                           (FStar_Sealed.seal
-                                                              (Obj.magic
-                                                                 (FStar_Range.mk_range
-                                                                    "Pulse.Checker.Abs.fst"
-                                                                    (Prims.of_int (109))
-                                                                    (Prims.of_int (73))
-                                                                    (Prims.of_int (111))
-                                                                    (Prims.of_int (65)))))
-                                                           (FStar_Tactics_Effect.lift_div_tac
-                                                              (fun uu___1 ->
-                                                                 {
-                                                                   Pulse_Syntax_Base.binder_ty
-                                                                    = ty1;
-                                                                   Pulse_Syntax_Base.binder_ppname
-                                                                    =
-                                                                    (b.Pulse_Syntax_Base.binder_ppname)
-                                                                 }))
-                                                           (fun uu___1 ->
-                                                              (fun b1 ->
-                                                                 Obj.magic
-                                                                   (FStar_Tactics_Effect.tac_bind
+                                       (fun uu___1 ->
+                                          Obj.magic
+                                            (FStar_Tactics_Effect.tac_bind
+                                               (FStar_Sealed.seal
+                                                  (Obj.magic
+                                                     (FStar_Range.mk_range
+                                                        "Pulse.Checker.Abs.fst"
+                                                        (Prims.of_int (108))
+                                                        (Prims.of_int (15))
+                                                        (Prims.of_int (108))
+                                                        (Prims.of_int (34)))))
+                                               (FStar_Sealed.seal
+                                                  (Obj.magic
+                                                     (FStar_Range.mk_range
+                                                        "Pulse.Checker.Abs.fst"
+                                                        (Prims.of_int (108))
+                                                        (Prims.of_int (37))
+                                                        (Prims.of_int (134))
+                                                        (Prims.of_int (41)))))
+                                               (FStar_Tactics_Effect.lift_div_tac
+                                                  (fun uu___2 ->
+                                                     Pulse_Readback.readback_ty
+                                                       b'1.FStar_Reflection_V2_Data.sort2))
+                                               (fun uu___2 ->
+                                                  (fun ty ->
+                                                     Obj.magic
+                                                       (FStar_Tactics_Effect.tac_bind
+                                                          (FStar_Sealed.seal
+                                                             (Obj.magic
+                                                                (FStar_Range.mk_range
+                                                                   "Pulse.Checker.Abs.fst"
+                                                                   (Prims.of_int (109))
+                                                                   (Prims.of_int (17))
+                                                                   (Prims.of_int (109))
+                                                                   (Prims.of_int (34)))))
+                                                          (FStar_Sealed.seal
+                                                             (Obj.magic
+                                                                (FStar_Range.mk_range
+                                                                   "Pulse.Checker.Abs.fst"
+                                                                   (Prims.of_int (110))
+                                                                   (Prims.of_int (6))
+                                                                   (Prims.of_int (134))
+                                                                   (Prims.of_int (41)))))
+                                                          (FStar_Tactics_Effect.lift_div_tac
+                                                             (fun uu___2 ->
+                                                                FStar_Reflection_V2_Builtins.inspect_comp
+                                                                  c'))
+                                                          (fun uu___2 ->
+                                                             (fun comp ->
+                                                                match 
+                                                                  (ty, comp)
+                                                                with
+                                                                | (FStar_Pervasives_Native.Some
+                                                                   ty1,
+                                                                   FStar_Reflection_V2_Data.C_Total
+                                                                   res_ty) ->
+                                                                    Obj.magic
+                                                                    (Obj.repr
+                                                                    (if
+                                                                    Pulse_Syntax_Base.uu___is_Tm_Abs
+                                                                    body.Pulse_Syntax_Base.term1
+                                                                    then
+                                                                    Obj.repr
+                                                                    (FStar_Tactics_Effect.tac_bind
                                                                     (FStar_Sealed.seal
                                                                     (Obj.magic
                                                                     (FStar_Range.mk_range
                                                                     "Pulse.Checker.Abs.fst"
-                                                                    (Prims.of_int (110))
+                                                                    (Prims.of_int (114))
+                                                                    (Prims.of_int (20))
+                                                                    (Prims.of_int (114))
+                                                                    (Prims.of_int (68)))))
+                                                                    (FStar_Sealed.seal
+                                                                    (Obj.magic
+                                                                    (FStar_Range.mk_range
+                                                                    "Pulse.Checker.Abs.fst"
+                                                                    (Prims.of_int (114))
+                                                                    (Prims.of_int (73))
+                                                                    (Prims.of_int (117))
+                                                                    (Prims.of_int (64)))))
+                                                                    (FStar_Tactics_Effect.lift_div_tac
+                                                                    (fun
+                                                                    uu___2 ->
+                                                                    {
+                                                                    Pulse_Syntax_Base.binder_ty
+                                                                    = ty1;
+                                                                    Pulse_Syntax_Base.binder_ppname
+                                                                    =
+                                                                    (b.Pulse_Syntax_Base.binder_ppname)
+                                                                    }))
+                                                                    (fun
+                                                                    uu___2 ->
+                                                                    (fun b1
+                                                                    ->
+                                                                    Obj.magic
+                                                                    (FStar_Tactics_Effect.tac_bind
+                                                                    (FStar_Sealed.seal
+                                                                    (Obj.magic
+                                                                    (FStar_Range.mk_range
+                                                                    "Pulse.Checker.Abs.fst"
+                                                                    (Prims.of_int (115))
                                                                     (Prims.of_int (21))
-                                                                    (Prims.of_int (110))
+                                                                    (Prims.of_int (115))
                                                                     (Prims.of_int (46)))))
                                                                     (FStar_Sealed.seal
                                                                     (Obj.magic
                                                                     (FStar_Range.mk_range
                                                                     "Pulse.Checker.Abs.fst"
-                                                                    (Prims.of_int (111))
+                                                                    (Prims.of_int (117))
                                                                     (Prims.of_int (12))
-                                                                    (Prims.of_int (111))
-                                                                    (Prims.of_int (64)))))
+                                                                    (Prims.of_int (117))
+                                                                    (Prims.of_int (63)))))
                                                                     (Obj.magic
                                                                     (rebuild_abs
                                                                     g body
@@ -749,7 +803,7 @@ let rec (rebuild_abs :
                                                                     body1 ->
                                                                     FStar_Tactics_Effect.lift_div_tac
                                                                     (fun
-                                                                    uu___1 ->
+                                                                    uu___2 ->
                                                                     {
                                                                     Pulse_Syntax_Base.term1
                                                                     =
@@ -761,7 +815,14 @@ let rec (rebuild_abs :
                                                                     = q;
                                                                     Pulse_Syntax_Base.ascription
                                                                     =
-                                                                    FStar_Pervasives_Native.None;
+                                                                    {
+                                                                    Pulse_Syntax_Base.annotated
+                                                                    =
+                                                                    (asc.Pulse_Syntax_Base.annotated);
+                                                                    Pulse_Syntax_Base.elaborated
+                                                                    =
+                                                                    FStar_Pervasives_Native.None
+                                                                    };
                                                                     Pulse_Syntax_Base.body
                                                                     = body1
                                                                     });
@@ -772,41 +833,43 @@ let rec (rebuild_abs :
                                                                     =
                                                                     (t.Pulse_Syntax_Base.effect_tag)
                                                                     }))))
-                                                                uu___1))
-                                                    else
-                                                      Obj.repr
-                                                        (match Pulse_Readback.readback_comp
-                                                                 res_ty
-                                                         with
-                                                         | FStar_Pervasives_Native.None
-                                                             ->
-                                                             Obj.repr
-                                                               (FStar_Tactics_Effect.tac_bind
-                                                                  (FStar_Sealed.seal
-                                                                    (Obj.magic
-                                                                    (FStar_Range.mk_range
-                                                                    "Pulse.Checker.Abs.fst"
-                                                                    (Prims.of_int (117))
-                                                                    (Prims.of_int (14))
-                                                                    (Prims.of_int (118))
-                                                                    (Prims.of_int (44)))))
-                                                                  (FStar_Sealed.seal
-                                                                    (Obj.magic
-                                                                    (FStar_Range.mk_range
-                                                                    "Pulse.Checker.Abs.fst"
-                                                                    (Prims.of_int (116))
-                                                                    (Prims.of_int (12))
-                                                                    (Prims.of_int (118))
-                                                                    (Prims.of_int (44)))))
-                                                                  (Obj.magic
+                                                                    uu___2))
+                                                                    else
+                                                                    Obj.repr
+                                                                    (match 
+                                                                    Pulse_Readback.readback_comp
+                                                                    res_ty
+                                                                    with
+                                                                    | 
+                                                                    FStar_Pervasives_Native.None
+                                                                    ->
+                                                                    Obj.repr
                                                                     (FStar_Tactics_Effect.tac_bind
                                                                     (FStar_Sealed.seal
                                                                     (Obj.magic
                                                                     (FStar_Range.mk_range
                                                                     "Pulse.Checker.Abs.fst"
-                                                                    (Prims.of_int (118))
+                                                                    (Prims.of_int (123))
+                                                                    (Prims.of_int (14))
+                                                                    (Prims.of_int (124))
+                                                                    (Prims.of_int (44)))))
+                                                                    (FStar_Sealed.seal
+                                                                    (Obj.magic
+                                                                    (FStar_Range.mk_range
+                                                                    "Pulse.Checker.Abs.fst"
+                                                                    (Prims.of_int (122))
+                                                                    (Prims.of_int (12))
+                                                                    (Prims.of_int (124))
+                                                                    (Prims.of_int (44)))))
+                                                                    (Obj.magic
+                                                                    (FStar_Tactics_Effect.tac_bind
+                                                                    (FStar_Sealed.seal
+                                                                    (Obj.magic
+                                                                    (FStar_Range.mk_range
+                                                                    "Pulse.Checker.Abs.fst"
+                                                                    (Prims.of_int (124))
                                                                     (Prims.of_int (18))
-                                                                    (Prims.of_int (118))
+                                                                    (Prims.of_int (124))
                                                                     (Prims.of_int (43)))))
                                                                     (FStar_Sealed.seal
                                                                     (Obj.magic
@@ -820,32 +883,33 @@ let rec (rebuild_abs :
                                                                     (FStar_Tactics_V2_Builtins.term_to_string
                                                                     res_ty))
                                                                     (fun
-                                                                    uu___2 ->
+                                                                    uu___3 ->
                                                                     FStar_Tactics_Effect.lift_div_tac
                                                                     (fun
-                                                                    uu___3 ->
+                                                                    uu___4 ->
                                                                     Prims.strcat
                                                                     "Expected a computation type; got "
                                                                     (Prims.strcat
-                                                                    uu___2 "")))))
-                                                                  (fun uu___2
-                                                                    ->
+                                                                    uu___3 "")))))
                                                                     (fun
-                                                                    uu___2 ->
+                                                                    uu___3 ->
+                                                                    (fun
+                                                                    uu___3 ->
                                                                     Obj.magic
                                                                     (Pulse_Typing_Env.fail
                                                                     g
                                                                     (FStar_Pervasives_Native.Some
                                                                     (FStar_Reflection_V2_Builtins.range_of_term
                                                                     res_ty))
-                                                                    uu___2))
-                                                                    uu___2))
-                                                         | FStar_Pervasives_Native.Some
-                                                             c ->
-                                                             Obj.repr
-                                                               (FStar_Tactics_Effect.lift_div_tac
-                                                                  (fun uu___2
-                                                                    ->
+                                                                    uu___3))
+                                                                    uu___3))
+                                                                    | 
+                                                                    FStar_Pervasives_Native.Some
+                                                                    c ->
+                                                                    Obj.repr
+                                                                    (FStar_Tactics_Effect.lift_div_tac
+                                                                    (fun
+                                                                    uu___3 ->
                                                                     {
                                                                     Pulse_Syntax_Base.term1
                                                                     =
@@ -864,14 +928,15 @@ let rec (rebuild_abs :
                                                                     = q;
                                                                     Pulse_Syntax_Base.ascription
                                                                     =
-                                                                    (FStar_Pervasives_Native.Some
                                                                     {
                                                                     Pulse_Syntax_Base.annotated
                                                                     =
-                                                                    FStar_Pervasives_Native.None;
+                                                                    (asc.Pulse_Syntax_Base.annotated);
                                                                     Pulse_Syntax_Base.elaborated
-                                                                    = c
-                                                                    });
+                                                                    =
+                                                                    (FStar_Pervasives_Native.Some
+                                                                    c)
+                                                                    };
                                                                     Pulse_Syntax_Base.body
                                                                     = body
                                                                     });
@@ -882,65 +947,69 @@ let rec (rebuild_abs :
                                                                     =
                                                                     (t.Pulse_Syntax_Base.effect_tag)
                                                                     })))))
-                                          | uu___1 ->
-                                              Obj.magic
-                                                (Obj.repr
-                                                   (FStar_Tactics_Effect.tac_bind
-                                                      (FStar_Sealed.seal
-                                                         (Obj.magic
-                                                            (FStar_Range.mk_range
-                                                               "Pulse.Checker.Abs.fst"
-                                                               (Prims.of_int (127))
-                                                               (Prims.of_int (12))
-                                                               (Prims.of_int (128))
-                                                               (Prims.of_int (41)))))
-                                                      (FStar_Sealed.seal
-                                                         (Obj.magic
-                                                            (FStar_Range.mk_range
-                                                               "Pulse.Checker.Abs.fst"
-                                                               (Prims.of_int (126))
-                                                               (Prims.of_int (8))
-                                                               (Prims.of_int (128))
-                                                               (Prims.of_int (41)))))
-                                                      (Obj.magic
-                                                         (FStar_Tactics_Effect.tac_bind
-                                                            (FStar_Sealed.seal
-                                                               (Obj.magic
-                                                                  (FStar_Range.mk_range
+                                                                | uu___2 ->
+                                                                    Obj.magic
+                                                                    (Obj.repr
+                                                                    (FStar_Tactics_Effect.tac_bind
+                                                                    (FStar_Sealed.seal
+                                                                    (Obj.magic
+                                                                    (FStar_Range.mk_range
                                                                     "Pulse.Checker.Abs.fst"
-                                                                    (Prims.of_int (128))
+                                                                    (Prims.of_int (133))
+                                                                    (Prims.of_int (12))
+                                                                    (Prims.of_int (134))
+                                                                    (Prims.of_int (41)))))
+                                                                    (FStar_Sealed.seal
+                                                                    (Obj.magic
+                                                                    (FStar_Range.mk_range
+                                                                    "Pulse.Checker.Abs.fst"
+                                                                    (Prims.of_int (132))
+                                                                    (Prims.of_int (8))
+                                                                    (Prims.of_int (134))
+                                                                    (Prims.of_int (41)))))
+                                                                    (Obj.magic
+                                                                    (FStar_Tactics_Effect.tac_bind
+                                                                    (FStar_Sealed.seal
+                                                                    (Obj.magic
+                                                                    (FStar_Range.mk_range
+                                                                    "Pulse.Checker.Abs.fst"
+                                                                    (Prims.of_int (134))
                                                                     (Prims.of_int (16))
-                                                                    (Prims.of_int (128))
+                                                                    (Prims.of_int (134))
                                                                     (Prims.of_int (40)))))
-                                                            (FStar_Sealed.seal
-                                                               (Obj.magic
-                                                                  (FStar_Range.mk_range
+                                                                    (FStar_Sealed.seal
+                                                                    (Obj.magic
+                                                                    (FStar_Range.mk_range
                                                                     "prims.fst"
                                                                     (Prims.of_int (590))
                                                                     (Prims.of_int (19))
                                                                     (Prims.of_int (590))
                                                                     (Prims.of_int (31)))))
-                                                            (Obj.magic
-                                                               (FStar_Tactics_V2_Builtins.term_to_string
-                                                                  annot))
-                                                            (fun uu___2 ->
-                                                               FStar_Tactics_Effect.lift_div_tac
-                                                                 (fun uu___3
-                                                                    ->
+                                                                    (Obj.magic
+                                                                    (FStar_Tactics_V2_Builtins.term_to_string
+                                                                    annot))
+                                                                    (fun
+                                                                    uu___3 ->
+                                                                    FStar_Tactics_Effect.lift_div_tac
+                                                                    (fun
+                                                                    uu___4 ->
                                                                     Prims.strcat
                                                                     "Unexpected type of abstraction: "
                                                                     (Prims.strcat
-                                                                    uu___2 "")))))
-                                                      (fun uu___2 ->
-                                                         (fun uu___2 ->
-                                                            Obj.magic
-                                                              (Pulse_Typing_Env.fail
-                                                                 g
-                                                                 (FStar_Pervasives_Native.Some
-                                                                    (
-                                                                    t.Pulse_Syntax_Base.range2))
-                                                                 uu___2))
-                                                           uu___2)))) uu___1)))
+                                                                    uu___3 "")))))
+                                                                    (fun
+                                                                    uu___3 ->
+                                                                    (fun
+                                                                    uu___3 ->
+                                                                    Obj.magic
+                                                                    (Pulse_Typing_Env.fail
+                                                                    g
+                                                                    (FStar_Pervasives_Native.Some
+                                                                    (t.Pulse_Syntax_Base.range2))
+                                                                    uu___3))
+                                                                    uu___3))))
+                                                               uu___2)))
+                                                    uu___2))) uu___1)))
                               uu___1))
                 | uu___1 ->
                     Obj.magic
@@ -948,22 +1017,22 @@ let rec (rebuild_abs :
                          (FStar_Sealed.seal
                             (Obj.magic
                                (FStar_Range.mk_range "Pulse.Checker.Abs.fst"
-                                  (Prims.of_int (153)) (Prims.of_int (16))
-                                  (Prims.of_int (154)) (Prims.of_int (47)))))
+                                  (Prims.of_int (159)) (Prims.of_int (16))
+                                  (Prims.of_int (160)) (Prims.of_int (47)))))
                          (FStar_Sealed.seal
                             (Obj.magic
                                (FStar_Range.mk_range "Pulse.Checker.Abs.fst"
-                                  (Prims.of_int (152)) (Prims.of_int (6))
-                                  (Prims.of_int (154)) (Prims.of_int (47)))))
+                                  (Prims.of_int (158)) (Prims.of_int (6))
+                                  (Prims.of_int (160)) (Prims.of_int (47)))))
                          (Obj.magic
                             (FStar_Tactics_Effect.tac_bind
                                (FStar_Sealed.seal
                                   (Obj.magic
                                      (FStar_Range.mk_range
                                         "Pulse.Checker.Abs.fst"
-                                        (Prims.of_int (154))
+                                        (Prims.of_int (160))
                                         (Prims.of_int (22))
-                                        (Prims.of_int (154))
+                                        (Prims.of_int (160))
                                         (Prims.of_int (46)))))
                                (FStar_Sealed.seal
                                   (Obj.magic
@@ -999,12 +1068,12 @@ let (preprocess_abs :
         (FStar_Sealed.seal
            (Obj.magic
               (FStar_Range.mk_range "Pulse.Checker.Abs.fst"
-                 (Prims.of_int (160)) (Prims.of_int (16))
-                 (Prims.of_int (160)) (Prims.of_int (32)))))
+                 (Prims.of_int (166)) (Prims.of_int (16))
+                 (Prims.of_int (166)) (Prims.of_int (32)))))
         (FStar_Sealed.seal
            (Obj.magic
               (FStar_Range.mk_range "Pulse.Checker.Abs.fst"
-                 (Prims.of_int (161)) (Prims.of_int (4)) (Prims.of_int (171))
+                 (Prims.of_int (167)) (Prims.of_int (4)) (Prims.of_int (177))
                  (Prims.of_int (51))))) (Obj.magic (arrow_of_abs g t))
         (fun uu___ ->
            (fun annot ->
@@ -1013,13 +1082,13 @@ let (preprocess_abs :
                    (FStar_Sealed.seal
                       (Obj.magic
                          (FStar_Range.mk_range "Pulse.Checker.Abs.fst"
-                            (Prims.of_int (161)) (Prims.of_int (4))
-                            (Prims.of_int (161)) (Prims.of_int (88)))))
+                            (Prims.of_int (167)) (Prims.of_int (4))
+                            (Prims.of_int (167)) (Prims.of_int (88)))))
                    (FStar_Sealed.seal
                       (Obj.magic
                          (FStar_Range.mk_range "Pulse.Checker.Abs.fst"
-                            (Prims.of_int (161)) (Prims.of_int (89))
-                            (Prims.of_int (171)) (Prims.of_int (51)))))
+                            (Prims.of_int (167)) (Prims.of_int (89))
+                            (Prims.of_int (177)) (Prims.of_int (51)))))
                    (Obj.magic
                       (debug_abs g
                          (fun uu___ ->
@@ -1028,9 +1097,9 @@ let (preprocess_abs :
                                  (Obj.magic
                                     (FStar_Range.mk_range
                                        "Pulse.Checker.Abs.fst"
-                                       (Prims.of_int (161))
+                                       (Prims.of_int (167))
                                        (Prims.of_int (63))
-                                       (Prims.of_int (161))
+                                       (Prims.of_int (167))
                                        (Prims.of_int (87)))))
                               (FStar_Sealed.seal
                                  (Obj.magic
@@ -1054,17 +1123,17 @@ let (preprocess_abs :
                                  (Obj.magic
                                     (FStar_Range.mk_range
                                        "Pulse.Checker.Abs.fst"
-                                       (Prims.of_int (162))
+                                       (Prims.of_int (168))
                                        (Prims.of_int (19))
-                                       (Prims.of_int (162))
+                                       (Prims.of_int (168))
                                        (Prims.of_int (72)))))
                               (FStar_Sealed.seal
                                  (Obj.magic
                                     (FStar_Range.mk_range
                                        "Pulse.Checker.Abs.fst"
-                                       (Prims.of_int (161))
+                                       (Prims.of_int (167))
                                        (Prims.of_int (89))
-                                       (Prims.of_int (171))
+                                       (Prims.of_int (177))
                                        (Prims.of_int (51)))))
                               (Obj.magic
                                  (Pulse_Checker_Pure.instantiate_term_implicits
@@ -1083,17 +1152,17 @@ let (preprocess_abs :
                                                      (Obj.magic
                                                         (FStar_Range.mk_range
                                                            "Pulse.Checker.Abs.fst"
-                                                           (Prims.of_int (165))
+                                                           (Prims.of_int (171))
                                                            (Prims.of_int (16))
-                                                           (Prims.of_int (165))
+                                                           (Prims.of_int (171))
                                                            (Prims.of_int (37)))))
                                                   (FStar_Sealed.seal
                                                      (Obj.magic
                                                         (FStar_Range.mk_range
                                                            "Pulse.Checker.Abs.fst"
-                                                           (Prims.of_int (166))
+                                                           (Prims.of_int (172))
                                                            (Prims.of_int (6))
-                                                           (Prims.of_int (167))
+                                                           (Prims.of_int (173))
                                                            (Prims.of_int (9)))))
                                                   (Obj.magic
                                                      (rebuild_abs g t annot2))
@@ -1105,17 +1174,17 @@ let (preprocess_abs :
                                                                 (Obj.magic
                                                                    (FStar_Range.mk_range
                                                                     "Pulse.Checker.Abs.fst"
-                                                                    (Prims.of_int (166))
+                                                                    (Prims.of_int (172))
                                                                     (Prims.of_int (6))
-                                                                    (Prims.of_int (166))
+                                                                    (Prims.of_int (172))
                                                                     (Prims.of_int (90)))))
                                                              (FStar_Sealed.seal
                                                                 (Obj.magic
                                                                    (FStar_Range.mk_range
                                                                     "Pulse.Checker.Abs.fst"
-                                                                    (Prims.of_int (165))
+                                                                    (Prims.of_int (171))
                                                                     (Prims.of_int (10))
-                                                                    (Prims.of_int (165))
+                                                                    (Prims.of_int (171))
                                                                     (Prims.of_int (13)))))
                                                              (Obj.magic
                                                                 (debug_abs g
@@ -1126,9 +1195,9 @@ let (preprocess_abs :
                                                                     (Obj.magic
                                                                     (FStar_Range.mk_range
                                                                     "Pulse.Checker.Abs.fst"
-                                                                    (Prims.of_int (166))
+                                                                    (Prims.of_int (172))
                                                                     (Prims.of_int (64))
-                                                                    (Prims.of_int (166))
+                                                                    (Prims.of_int (172))
                                                                     (Prims.of_int (89)))))
                                                                     (FStar_Sealed.seal
                                                                     (Obj.magic
@@ -1163,17 +1232,17 @@ let (preprocess_abs :
                                                      (Obj.magic
                                                         (FStar_Range.mk_range
                                                            "Pulse.Checker.Abs.fst"
-                                                           (Prims.of_int (170))
+                                                           (Prims.of_int (176))
                                                            (Prims.of_int (17))
-                                                           (Prims.of_int (171))
+                                                           (Prims.of_int (177))
                                                            (Prims.of_int (51)))))
                                                   (FStar_Sealed.seal
                                                      (Obj.magic
                                                         (FStar_Range.mk_range
                                                            "Pulse.Checker.Abs.fst"
-                                                           (Prims.of_int (169))
+                                                           (Prims.of_int (175))
                                                            (Prims.of_int (6))
-                                                           (Prims.of_int (171))
+                                                           (Prims.of_int (177))
                                                            (Prims.of_int (51)))))
                                                   (Obj.magic
                                                      (FStar_Tactics_Effect.tac_bind
@@ -1181,9 +1250,9 @@ let (preprocess_abs :
                                                            (Obj.magic
                                                               (FStar_Range.mk_range
                                                                  "Pulse.Checker.Abs.fst"
-                                                                 (Prims.of_int (171))
+                                                                 (Prims.of_int (177))
                                                                  (Prims.of_int (26))
-                                                                 (Prims.of_int (171))
+                                                                 (Prims.of_int (177))
                                                                  (Prims.of_int (50)))))
                                                         (FStar_Sealed.seal
                                                            (Obj.magic
@@ -1215,7 +1284,7 @@ let (preprocess_abs :
 let (check_effect_annotation :
   Pulse_Typing_Env.env ->
     Pulse_Syntax_Base.range ->
-      Pulse_Syntax_Base.comp_ascription FStar_Pervasives_Native.option ->
+      Pulse_Syntax_Base.comp_ascription ->
         Pulse_Syntax_Base.comp -> (unit, unit) FStar_Tactics_Effect.tac_repr)
   =
   fun uu___3 ->
@@ -1224,39 +1293,36 @@ let (check_effect_annotation :
         fun uu___ ->
           (fun g ->
              fun r ->
-               fun c_annot ->
+               fun asc ->
                  fun c_computed ->
-                   match c_annot with
+                   match asc.Pulse_Syntax_Base.elaborated with
                    | FStar_Pervasives_Native.None ->
                        Obj.magic
                          (Obj.repr
                             (FStar_Tactics_Effect.lift_div_tac
                                (fun uu___ -> ())))
-                   | FStar_Pervasives_Native.Some
-                       { Pulse_Syntax_Base.annotated = uu___;
-                         Pulse_Syntax_Base.elaborated = c_annot1;_}
-                       ->
+                   | FStar_Pervasives_Native.Some c ->
                        Obj.magic
                          (Obj.repr
-                            (match (c_annot1, c_computed) with
-                             | (Pulse_Syntax_Base.C_Tot uu___1,
-                                Pulse_Syntax_Base.C_Tot uu___2) ->
+                            (match (c, c_computed) with
+                             | (Pulse_Syntax_Base.C_Tot uu___,
+                                Pulse_Syntax_Base.C_Tot uu___1) ->
                                  Obj.repr
                                    (FStar_Tactics_Effect.lift_div_tac
-                                      (fun uu___3 -> ()))
-                             | (Pulse_Syntax_Base.C_ST uu___1,
-                                Pulse_Syntax_Base.C_ST uu___2) ->
+                                      (fun uu___2 -> ()))
+                             | (Pulse_Syntax_Base.C_ST uu___,
+                                Pulse_Syntax_Base.C_ST uu___1) ->
                                  Obj.repr
                                    (FStar_Tactics_Effect.lift_div_tac
-                                      (fun uu___3 -> ()))
-                             | (Pulse_Syntax_Base.C_STAtomic (i, uu___1),
-                                Pulse_Syntax_Base.C_STAtomic (j, uu___2)) ->
+                                      (fun uu___2 -> ()))
+                             | (Pulse_Syntax_Base.C_STAtomic (i, uu___),
+                                Pulse_Syntax_Base.C_STAtomic (j, uu___1)) ->
                                  Obj.repr
                                    (if Pulse_Syntax_Base.eq_tm i j
                                     then
                                       Obj.repr
                                         (FStar_Tactics_Effect.lift_div_tac
-                                           (fun uu___3 -> ()))
+                                           (fun uu___2 -> ()))
                                     else
                                       Obj.repr
                                         (FStar_Tactics_Effect.tac_bind
@@ -1264,17 +1330,17 @@ let (check_effect_annotation :
                                               (Obj.magic
                                                  (FStar_Range.mk_range
                                                     "Pulse.Checker.Abs.fst"
-                                                    (Prims.of_int (185))
+                                                    (Prims.of_int (191))
                                                     (Prims.of_int (18))
-                                                    (Prims.of_int (187))
+                                                    (Prims.of_int (193))
                                                     (Prims.of_int (41)))))
                                            (FStar_Sealed.seal
                                               (Obj.magic
                                                  (FStar_Range.mk_range
                                                     "Pulse.Checker.Abs.fst"
-                                                    (Prims.of_int (184))
+                                                    (Prims.of_int (190))
                                                     (Prims.of_int (11))
-                                                    (Prims.of_int (187))
+                                                    (Prims.of_int (193))
                                                     (Prims.of_int (41)))))
                                            (Obj.magic
                                               (FStar_Tactics_Effect.tac_bind
@@ -1282,40 +1348,40 @@ let (check_effect_annotation :
                                                     (Obj.magic
                                                        (FStar_Range.mk_range
                                                           "Pulse.Checker.Abs.fst"
-                                                          (Prims.of_int (187))
+                                                          (Prims.of_int (193))
                                                           (Prims.of_int (20))
-                                                          (Prims.of_int (187))
+                                                          (Prims.of_int (193))
                                                           (Prims.of_int (40)))))
                                                  (FStar_Sealed.seal
                                                     (Obj.magic
                                                        (FStar_Range.mk_range
                                                           "Pulse.Checker.Abs.fst"
-                                                          (Prims.of_int (185))
+                                                          (Prims.of_int (191))
                                                           (Prims.of_int (18))
-                                                          (Prims.of_int (187))
+                                                          (Prims.of_int (193))
                                                           (Prims.of_int (41)))))
                                                  (Obj.magic
                                                     (Pulse_Syntax_Printer.term_to_string
                                                        j))
-                                                 (fun uu___4 ->
-                                                    (fun uu___4 ->
+                                                 (fun uu___3 ->
+                                                    (fun uu___3 ->
                                                        Obj.magic
                                                          (FStar_Tactics_Effect.tac_bind
                                                             (FStar_Sealed.seal
                                                                (Obj.magic
                                                                   (FStar_Range.mk_range
                                                                     "Pulse.Checker.Abs.fst"
-                                                                    (Prims.of_int (185))
+                                                                    (Prims.of_int (191))
                                                                     (Prims.of_int (18))
-                                                                    (Prims.of_int (187))
+                                                                    (Prims.of_int (193))
                                                                     (Prims.of_int (41)))))
                                                             (FStar_Sealed.seal
                                                                (Obj.magic
                                                                   (FStar_Range.mk_range
                                                                     "Pulse.Checker.Abs.fst"
-                                                                    (Prims.of_int (185))
+                                                                    (Prims.of_int (191))
                                                                     (Prims.of_int (18))
-                                                                    (Prims.of_int (187))
+                                                                    (Prims.of_int (193))
                                                                     (Prims.of_int (41)))))
                                                             (Obj.magic
                                                                (FStar_Tactics_Effect.tac_bind
@@ -1323,9 +1389,9 @@ let (check_effect_annotation :
                                                                     (Obj.magic
                                                                     (FStar_Range.mk_range
                                                                     "Pulse.Checker.Abs.fst"
-                                                                    (Prims.of_int (186))
+                                                                    (Prims.of_int (192))
                                                                     (Prims.of_int (20))
-                                                                    (Prims.of_int (186))
+                                                                    (Prims.of_int (192))
                                                                     (Prims.of_int (40)))))
                                                                   (FStar_Sealed.seal
                                                                     (Obj.magic
@@ -1338,43 +1404,43 @@ let (check_effect_annotation :
                                                                   (Obj.magic
                                                                     (Pulse_Syntax_Printer.term_to_string
                                                                     i))
-                                                                  (fun uu___5
+                                                                  (fun uu___4
                                                                     ->
                                                                     FStar_Tactics_Effect.lift_div_tac
                                                                     (fun
-                                                                    uu___6 ->
+                                                                    uu___5 ->
                                                                     fun x ->
                                                                     Prims.strcat
                                                                     (Prims.strcat
                                                                     "Annotated effect expects only invariants in "
                                                                     (Prims.strcat
-                                                                    uu___5
+                                                                    uu___4
                                                                     " to be opened; but computed effect claims that invariants "))
                                                                     (Prims.strcat
                                                                     x
                                                                     " are opened")))))
-                                                            (fun uu___5 ->
+                                                            (fun uu___4 ->
                                                                FStar_Tactics_Effect.lift_div_tac
-                                                                 (fun uu___6
+                                                                 (fun uu___5
                                                                     ->
-                                                                    uu___5
-                                                                    uu___4))))
-                                                      uu___4)))
-                                           (fun uu___4 ->
-                                              (fun uu___4 ->
+                                                                    uu___4
+                                                                    uu___3))))
+                                                      uu___3)))
+                                           (fun uu___3 ->
+                                              (fun uu___3 ->
                                                  Obj.magic
                                                    (Pulse_Typing_Env.fail g
                                                       (FStar_Pervasives_Native.Some
                                                          (i.Pulse_Syntax_Base.range1))
-                                                      uu___4)) uu___4)))
-                             | (Pulse_Syntax_Base.C_STGhost (i, uu___1),
-                                Pulse_Syntax_Base.C_STGhost (j, uu___2)) ->
+                                                      uu___3)) uu___3)))
+                             | (Pulse_Syntax_Base.C_STGhost (i, uu___),
+                                Pulse_Syntax_Base.C_STGhost (j, uu___1)) ->
                                  Obj.repr
                                    (if Pulse_Syntax_Base.eq_tm i j
                                     then
                                       Obj.repr
                                         (FStar_Tactics_Effect.lift_div_tac
-                                           (fun uu___3 -> ()))
+                                           (fun uu___2 -> ()))
                                     else
                                       Obj.repr
                                         (FStar_Tactics_Effect.tac_bind
@@ -1382,17 +1448,17 @@ let (check_effect_annotation :
                                               (Obj.magic
                                                  (FStar_Range.mk_range
                                                     "Pulse.Checker.Abs.fst"
-                                                    (Prims.of_int (185))
+                                                    (Prims.of_int (191))
                                                     (Prims.of_int (18))
-                                                    (Prims.of_int (187))
+                                                    (Prims.of_int (193))
                                                     (Prims.of_int (41)))))
                                            (FStar_Sealed.seal
                                               (Obj.magic
                                                  (FStar_Range.mk_range
                                                     "Pulse.Checker.Abs.fst"
-                                                    (Prims.of_int (184))
+                                                    (Prims.of_int (190))
                                                     (Prims.of_int (11))
-                                                    (Prims.of_int (187))
+                                                    (Prims.of_int (193))
                                                     (Prims.of_int (41)))))
                                            (Obj.magic
                                               (FStar_Tactics_Effect.tac_bind
@@ -1400,40 +1466,40 @@ let (check_effect_annotation :
                                                     (Obj.magic
                                                        (FStar_Range.mk_range
                                                           "Pulse.Checker.Abs.fst"
-                                                          (Prims.of_int (187))
+                                                          (Prims.of_int (193))
                                                           (Prims.of_int (20))
-                                                          (Prims.of_int (187))
+                                                          (Prims.of_int (193))
                                                           (Prims.of_int (40)))))
                                                  (FStar_Sealed.seal
                                                     (Obj.magic
                                                        (FStar_Range.mk_range
                                                           "Pulse.Checker.Abs.fst"
-                                                          (Prims.of_int (185))
+                                                          (Prims.of_int (191))
                                                           (Prims.of_int (18))
-                                                          (Prims.of_int (187))
+                                                          (Prims.of_int (193))
                                                           (Prims.of_int (41)))))
                                                  (Obj.magic
                                                     (Pulse_Syntax_Printer.term_to_string
                                                        j))
-                                                 (fun uu___4 ->
-                                                    (fun uu___4 ->
+                                                 (fun uu___3 ->
+                                                    (fun uu___3 ->
                                                        Obj.magic
                                                          (FStar_Tactics_Effect.tac_bind
                                                             (FStar_Sealed.seal
                                                                (Obj.magic
                                                                   (FStar_Range.mk_range
                                                                     "Pulse.Checker.Abs.fst"
-                                                                    (Prims.of_int (185))
+                                                                    (Prims.of_int (191))
                                                                     (Prims.of_int (18))
-                                                                    (Prims.of_int (187))
+                                                                    (Prims.of_int (193))
                                                                     (Prims.of_int (41)))))
                                                             (FStar_Sealed.seal
                                                                (Obj.magic
                                                                   (FStar_Range.mk_range
                                                                     "Pulse.Checker.Abs.fst"
-                                                                    (Prims.of_int (185))
+                                                                    (Prims.of_int (191))
                                                                     (Prims.of_int (18))
-                                                                    (Prims.of_int (187))
+                                                                    (Prims.of_int (193))
                                                                     (Prims.of_int (41)))))
                                                             (Obj.magic
                                                                (FStar_Tactics_Effect.tac_bind
@@ -1441,9 +1507,9 @@ let (check_effect_annotation :
                                                                     (Obj.magic
                                                                     (FStar_Range.mk_range
                                                                     "Pulse.Checker.Abs.fst"
-                                                                    (Prims.of_int (186))
+                                                                    (Prims.of_int (192))
                                                                     (Prims.of_int (20))
-                                                                    (Prims.of_int (186))
+                                                                    (Prims.of_int (192))
                                                                     (Prims.of_int (40)))))
                                                                   (FStar_Sealed.seal
                                                                     (Obj.magic
@@ -1456,53 +1522,53 @@ let (check_effect_annotation :
                                                                   (Obj.magic
                                                                     (Pulse_Syntax_Printer.term_to_string
                                                                     i))
-                                                                  (fun uu___5
+                                                                  (fun uu___4
                                                                     ->
                                                                     FStar_Tactics_Effect.lift_div_tac
                                                                     (fun
-                                                                    uu___6 ->
+                                                                    uu___5 ->
                                                                     fun x ->
                                                                     Prims.strcat
                                                                     (Prims.strcat
                                                                     "Annotated effect expects only invariants in "
                                                                     (Prims.strcat
-                                                                    uu___5
+                                                                    uu___4
                                                                     " to be opened; but computed effect claims that invariants "))
                                                                     (Prims.strcat
                                                                     x
                                                                     " are opened")))))
-                                                            (fun uu___5 ->
+                                                            (fun uu___4 ->
                                                                FStar_Tactics_Effect.lift_div_tac
-                                                                 (fun uu___6
+                                                                 (fun uu___5
                                                                     ->
-                                                                    uu___5
-                                                                    uu___4))))
-                                                      uu___4)))
-                                           (fun uu___4 ->
-                                              (fun uu___4 ->
+                                                                    uu___4
+                                                                    uu___3))))
+                                                      uu___3)))
+                                           (fun uu___3 ->
+                                              (fun uu___3 ->
                                                  Obj.magic
                                                    (Pulse_Typing_Env.fail g
                                                       (FStar_Pervasives_Native.Some
                                                          (i.Pulse_Syntax_Base.range1))
-                                                      uu___4)) uu___4)))
-                             | (uu___1, uu___2) ->
+                                                      uu___3)) uu___3)))
+                             | (uu___, uu___1) ->
                                  Obj.repr
                                    (FStar_Tactics_Effect.tac_bind
                                       (FStar_Sealed.seal
                                          (Obj.magic
                                             (FStar_Range.mk_range
                                                "Pulse.Checker.Abs.fst"
-                                               (Prims.of_int (190))
+                                               (Prims.of_int (196))
                                                (Prims.of_int (12))
-                                               (Prims.of_int (192))
+                                               (Prims.of_int (198))
                                                (Prims.of_int (47)))))
                                       (FStar_Sealed.seal
                                          (Obj.magic
                                             (FStar_Range.mk_range
                                                "Pulse.Checker.Abs.fst"
-                                               (Prims.of_int (189))
+                                               (Prims.of_int (195))
                                                (Prims.of_int (6))
-                                               (Prims.of_int (192))
+                                               (Prims.of_int (198))
                                                (Prims.of_int (47)))))
                                       (Obj.magic
                                          (FStar_Tactics_Effect.tac_bind
@@ -1510,40 +1576,40 @@ let (check_effect_annotation :
                                                (Obj.magic
                                                   (FStar_Range.mk_range
                                                      "Pulse.Checker.Abs.fst"
-                                                     (Prims.of_int (192))
+                                                     (Prims.of_int (198))
                                                      (Prims.of_int (20))
-                                                     (Prims.of_int (192))
+                                                     (Prims.of_int (198))
                                                      (Prims.of_int (46)))))
                                             (FStar_Sealed.seal
                                                (Obj.magic
                                                   (FStar_Range.mk_range
                                                      "Pulse.Checker.Abs.fst"
-                                                     (Prims.of_int (190))
+                                                     (Prims.of_int (196))
                                                      (Prims.of_int (12))
-                                                     (Prims.of_int (192))
+                                                     (Prims.of_int (198))
                                                      (Prims.of_int (47)))))
                                             (Obj.magic
                                                (Pulse_Syntax_Printer.tag_of_comp
                                                   c_computed))
-                                            (fun uu___3 ->
-                                               (fun uu___3 ->
+                                            (fun uu___2 ->
+                                               (fun uu___2 ->
                                                   Obj.magic
                                                     (FStar_Tactics_Effect.tac_bind
                                                        (FStar_Sealed.seal
                                                           (Obj.magic
                                                              (FStar_Range.mk_range
                                                                 "Pulse.Checker.Abs.fst"
-                                                                (Prims.of_int (190))
+                                                                (Prims.of_int (196))
                                                                 (Prims.of_int (12))
-                                                                (Prims.of_int (192))
+                                                                (Prims.of_int (198))
                                                                 (Prims.of_int (47)))))
                                                        (FStar_Sealed.seal
                                                           (Obj.magic
                                                              (FStar_Range.mk_range
                                                                 "Pulse.Checker.Abs.fst"
-                                                                (Prims.of_int (190))
+                                                                (Prims.of_int (196))
                                                                 (Prims.of_int (12))
-                                                                (Prims.of_int (192))
+                                                                (Prims.of_int (198))
                                                                 (Prims.of_int (47)))))
                                                        (Obj.magic
                                                           (FStar_Tactics_Effect.tac_bind
@@ -1551,10 +1617,10 @@ let (check_effect_annotation :
                                                                 (Obj.magic
                                                                    (FStar_Range.mk_range
                                                                     "Pulse.Checker.Abs.fst"
-                                                                    (Prims.of_int (191))
+                                                                    (Prims.of_int (197))
                                                                     (Prims.of_int (20))
-                                                                    (Prims.of_int (191))
-                                                                    (Prims.of_int (43)))))
+                                                                    (Prims.of_int (197))
+                                                                    (Prims.of_int (37)))))
                                                              (FStar_Sealed.seal
                                                                 (Obj.magic
                                                                    (FStar_Range.mk_range
@@ -1565,31 +1631,31 @@ let (check_effect_annotation :
                                                                     (Prims.of_int (44)))))
                                                              (Obj.magic
                                                                 (Pulse_Syntax_Printer.tag_of_comp
-                                                                   c_annot1))
-                                                             (fun uu___4 ->
+                                                                   c))
+                                                             (fun uu___3 ->
                                                                 FStar_Tactics_Effect.lift_div_tac
-                                                                  (fun uu___5
+                                                                  (fun uu___4
                                                                     ->
                                                                     fun x ->
                                                                     Prims.strcat
                                                                     (Prims.strcat
                                                                     "Expected effect "
                                                                     (Prims.strcat
-                                                                    uu___4
+                                                                    uu___3
                                                                     " but this function body has effect "))
                                                                     (Prims.strcat
                                                                     x "")))))
-                                                       (fun uu___4 ->
+                                                       (fun uu___3 ->
                                                           FStar_Tactics_Effect.lift_div_tac
-                                                            (fun uu___5 ->
-                                                               uu___4 uu___3))))
-                                                 uu___3)))
-                                      (fun uu___3 ->
-                                         (fun uu___3 ->
+                                                            (fun uu___4 ->
+                                                               uu___3 uu___2))))
+                                                 uu___2)))
+                                      (fun uu___2 ->
+                                         (fun uu___2 ->
                                             Obj.magic
                                               (Pulse_Typing_Env.fail g
                                                  (FStar_Pervasives_Native.Some
-                                                    r) uu___3)) uu___3)))))
+                                                    r) uu___2)) uu___2)))))
             uu___3 uu___2 uu___1 uu___
 let rec (check_abs_core :
   Pulse_Typing_Env.env ->
@@ -1607,13 +1673,13 @@ let rec (check_abs_core :
           (FStar_Sealed.seal
              (Obj.magic
                 (FStar_Range.mk_range "Pulse.Checker.Abs.fst"
-                   (Prims.of_int (201)) (Prims.of_int (14))
-                   (Prims.of_int (201)) (Prims.of_int (21)))))
+                   (Prims.of_int (207)) (Prims.of_int (14))
+                   (Prims.of_int (207)) (Prims.of_int (21)))))
           (FStar_Sealed.seal
              (Obj.magic
                 (FStar_Range.mk_range "Pulse.Checker.Abs.fst"
-                   (Prims.of_int (202)) (Prims.of_int (2))
-                   (Prims.of_int (273)) (Prims.of_int (29)))))
+                   (Prims.of_int (208)) (Prims.of_int (2))
+                   (Prims.of_int (279)) (Prims.of_int (29)))))
           (FStar_Tactics_Effect.lift_div_tac
              (fun uu___ -> t.Pulse_Syntax_Base.range2))
           (fun uu___ ->
@@ -1633,13 +1699,13 @@ let rec (check_abs_core :
                          (FStar_Sealed.seal
                             (Obj.magic
                                (FStar_Range.mk_range "Pulse.Checker.Abs.fst"
-                                  (Prims.of_int (206)) (Prims.of_int (24))
-                                  (Prims.of_int (206)) (Prims.of_int (42)))))
+                                  (Prims.of_int (212)) (Prims.of_int (24))
+                                  (Prims.of_int (212)) (Prims.of_int (42)))))
                          (FStar_Sealed.seal
                             (Obj.magic
                                (FStar_Range.mk_range "Pulse.Checker.Abs.fst"
-                                  (Prims.of_int (203)) (Prims.of_int (84))
-                                  (Prims.of_int (273)) (Prims.of_int (29)))))
+                                  (Prims.of_int (209)) (Prims.of_int (84))
+                                  (Prims.of_int (279)) (Prims.of_int (29)))))
                          (Obj.magic (Pulse_Checker_Pure.check_tot_term g t1))
                          (fun uu___ ->
                             (fun uu___ ->
@@ -1652,17 +1718,17 @@ let rec (check_abs_core :
                                            (Obj.magic
                                               (FStar_Range.mk_range
                                                  "Pulse.Checker.Abs.fst"
-                                                 (Prims.of_int (207))
+                                                 (Prims.of_int (213))
                                                  (Prims.of_int (28))
-                                                 (Prims.of_int (207))
+                                                 (Prims.of_int (213))
                                                  (Prims.of_int (46)))))
                                         (FStar_Sealed.seal
                                            (Obj.magic
                                               (FStar_Range.mk_range
                                                  "Pulse.Checker.Abs.fst"
-                                                 (Prims.of_int (206))
+                                                 (Prims.of_int (212))
                                                  (Prims.of_int (45))
-                                                 (Prims.of_int (273))
+                                                 (Prims.of_int (279))
                                                  (Prims.of_int (29)))))
                                         (Obj.magic
                                            (Pulse_Checker_Pure.check_universe
@@ -1678,17 +1744,17 @@ let rec (check_abs_core :
                                                           (Obj.magic
                                                              (FStar_Range.mk_range
                                                                 "Pulse.Checker.Abs.fst"
-                                                                (Prims.of_int (208))
+                                                                (Prims.of_int (214))
                                                                 (Prims.of_int (12))
-                                                                (Prims.of_int (208))
+                                                                (Prims.of_int (214))
                                                                 (Prims.of_int (19)))))
                                                        (FStar_Sealed.seal
                                                           (Obj.magic
                                                              (FStar_Range.mk_range
                                                                 "Pulse.Checker.Abs.fst"
-                                                                (Prims.of_int (208))
+                                                                (Prims.of_int (214))
                                                                 (Prims.of_int (22))
-                                                                (Prims.of_int (273))
+                                                                (Prims.of_int (279))
                                                                 (Prims.of_int (29)))))
                                                        (FStar_Tactics_Effect.lift_div_tac
                                                           (fun uu___4 ->
@@ -1702,17 +1768,17 @@ let rec (check_abs_core :
                                                                     (Obj.magic
                                                                     (FStar_Range.mk_range
                                                                     "Pulse.Checker.Abs.fst"
-                                                                    (Prims.of_int (209))
+                                                                    (Prims.of_int (215))
                                                                     (Prims.of_int (13))
-                                                                    (Prims.of_int (209))
+                                                                    (Prims.of_int (215))
                                                                     (Prims.of_int (22)))))
                                                                   (FStar_Sealed.seal
                                                                     (Obj.magic
                                                                     (FStar_Range.mk_range
                                                                     "Pulse.Checker.Abs.fst"
-                                                                    (Prims.of_int (209))
+                                                                    (Prims.of_int (215))
                                                                     (Prims.of_int (25))
-                                                                    (Prims.of_int (273))
+                                                                    (Prims.of_int (279))
                                                                     (Prims.of_int (29)))))
                                                                   (FStar_Tactics_Effect.lift_div_tac
                                                                     (fun
@@ -1729,17 +1795,17 @@ let rec (check_abs_core :
                                                                     (Obj.magic
                                                                     (FStar_Range.mk_range
                                                                     "Pulse.Checker.Abs.fst"
-                                                                    (Prims.of_int (210))
+                                                                    (Prims.of_int (216))
                                                                     (Prims.of_int (14))
-                                                                    (Prims.of_int (210))
+                                                                    (Prims.of_int (216))
                                                                     (Prims.of_int (50)))))
                                                                     (FStar_Sealed.seal
                                                                     (Obj.magic
                                                                     (FStar_Range.mk_range
                                                                     "Pulse.Checker.Abs.fst"
-                                                                    (Prims.of_int (210))
+                                                                    (Prims.of_int (216))
                                                                     (Prims.of_int (53))
-                                                                    (Prims.of_int (273))
+                                                                    (Prims.of_int (279))
                                                                     (Prims.of_int (29)))))
                                                                     (FStar_Tactics_Effect.lift_div_tac
                                                                     (fun
@@ -1761,17 +1827,17 @@ let rec (check_abs_core :
                                                                     (Obj.magic
                                                                     (FStar_Range.mk_range
                                                                     "Pulse.Checker.Abs.fst"
-                                                                    (Prims.of_int (211))
+                                                                    (Prims.of_int (217))
                                                                     (Prims.of_int (13))
-                                                                    (Prims.of_int (211))
+                                                                    (Prims.of_int (217))
                                                                     (Prims.of_int (38)))))
                                                                     (FStar_Sealed.seal
                                                                     (Obj.magic
                                                                     (FStar_Range.mk_range
                                                                     "Pulse.Checker.Abs.fst"
-                                                                    (Prims.of_int (211))
+                                                                    (Prims.of_int (217))
                                                                     (Prims.of_int (41))
-                                                                    (Prims.of_int (273))
+                                                                    (Prims.of_int (279))
                                                                     (Prims.of_int (29)))))
                                                                     (FStar_Tactics_Effect.lift_div_tac
                                                                     (fun
@@ -1789,17 +1855,17 @@ let rec (check_abs_core :
                                                                     (Obj.magic
                                                                     (FStar_Range.mk_range
                                                                     "Pulse.Checker.Abs.fst"
-                                                                    (Prims.of_int (212))
+                                                                    (Prims.of_int (218))
                                                                     (Prims.of_int (22))
-                                                                    (Prims.of_int (212))
+                                                                    (Prims.of_int (218))
                                                                     (Prims.of_int (45)))))
                                                                     (FStar_Sealed.seal
                                                                     (Obj.magic
                                                                     (FStar_Range.mk_range
                                                                     "Pulse.Checker.Abs.fst"
-                                                                    (Prims.of_int (213))
+                                                                    (Prims.of_int (219))
                                                                     (Prims.of_int (4))
-                                                                    (Prims.of_int (273))
+                                                                    (Prims.of_int (279))
                                                                     (Prims.of_int (29)))))
                                                                     (FStar_Tactics_Effect.lift_div_tac
                                                                     (fun
@@ -1823,17 +1889,17 @@ let rec (check_abs_core :
                                                                     (Obj.magic
                                                                     (FStar_Range.mk_range
                                                                     "Pulse.Checker.Abs.fst"
-                                                                    (Prims.of_int (215))
+                                                                    (Prims.of_int (221))
                                                                     (Prims.of_int (44))
-                                                                    (Prims.of_int (215))
+                                                                    (Prims.of_int (221))
                                                                     (Prims.of_int (79)))))
                                                                     (FStar_Sealed.seal
                                                                     (Obj.magic
                                                                     (FStar_Range.mk_range
                                                                     "Pulse.Checker.Abs.fst"
-                                                                    (Prims.of_int (214))
+                                                                    (Prims.of_int (220))
                                                                     (Prims.of_int (17))
-                                                                    (Prims.of_int (223))
+                                                                    (Prims.of_int (229))
                                                                     (Prims.of_int (29)))))
                                                                     (Obj.magic
                                                                     (check_abs_core
@@ -1858,17 +1924,17 @@ let rec (check_abs_core :
                                                                     (Obj.magic
                                                                     (FStar_Range.mk_range
                                                                     "Pulse.Checker.Abs.fst"
-                                                                    (Prims.of_int (216))
+                                                                    (Prims.of_int (222))
                                                                     (Prims.of_int (6))
-                                                                    (Prims.of_int (216))
+                                                                    (Prims.of_int (222))
                                                                     (Prims.of_int (52)))))
                                                                     (FStar_Sealed.seal
                                                                     (Obj.magic
                                                                     (FStar_Range.mk_range
                                                                     "Pulse.Checker.Abs.fst"
-                                                                    (Prims.of_int (223))
+                                                                    (Prims.of_int (229))
                                                                     (Prims.of_int (6))
-                                                                    (Prims.of_int (223))
+                                                                    (Prims.of_int (229))
                                                                     (Prims.of_int (29)))))
                                                                     (Obj.magic
                                                                     (check_effect_annotation
@@ -1897,7 +1963,7 @@ let rec (check_abs_core :
                                                                     = qual;
                                                                     Pulse_Syntax_Base.ascription
                                                                     =
-                                                                    FStar_Pervasives_Native.None;
+                                                                    Pulse_Syntax_Base.empty_ascription;
                                                                     Pulse_Syntax_Base.body
                                                                     =
                                                                     (Pulse_Syntax_Naming.close_st_term
@@ -1936,19 +2002,20 @@ let rec (check_abs_core :
                                                                     (Obj.magic
                                                                     (FStar_Range.mk_range
                                                                     "Pulse.Checker.Abs.fst"
-                                                                    (Prims.of_int (226))
+                                                                    (Prims.of_int (232))
                                                                     (Prims.of_int (8))
-                                                                    (Prims.of_int (241))
+                                                                    (Prims.of_int (247))
                                                                     (Prims.of_int (47)))))
                                                                     (FStar_Sealed.seal
                                                                     (Obj.magic
                                                                     (FStar_Range.mk_range
                                                                     "Pulse.Checker.Abs.fst"
-                                                                    (Prims.of_int (224))
+                                                                    (Prims.of_int (230))
                                                                     (Prims.of_int (10))
-                                                                    (Prims.of_int (273))
+                                                                    (Prims.of_int (279))
                                                                     (Prims.of_int (29)))))
-                                                                    (match c
+                                                                    (match 
+                                                                    c.Pulse_Syntax_Base.elaborated
                                                                     with
                                                                     | 
                                                                     FStar_Pervasives_Native.None
@@ -1962,13 +2029,8 @@ let rec (check_abs_core :
                                                                     "Missing annotation on a function body"))
                                                                     | 
                                                                     FStar_Pervasives_Native.Some
-                                                                    {
-                                                                    Pulse_Syntax_Base.annotated
-                                                                    = uu___5;
-                                                                    Pulse_Syntax_Base.elaborated
-                                                                    =
-                                                                    Pulse_Syntax_Base.C_Tot
-                                                                    r;_} ->
+                                                                    (Pulse_Syntax_Base.C_Tot
+                                                                    r) ->
                                                                     Obj.magic
                                                                     (Obj.repr
                                                                     (FStar_Tactics_Effect.tac_bind
@@ -1976,17 +2038,17 @@ let rec (check_abs_core :
                                                                     (Obj.magic
                                                                     (FStar_Range.mk_range
                                                                     "Pulse.Checker.Abs.fst"
-                                                                    (Prims.of_int (233))
+                                                                    (Prims.of_int (239))
                                                                     (Prims.of_int (12))
-                                                                    (Prims.of_int (235))
+                                                                    (Prims.of_int (241))
                                                                     (Prims.of_int (43)))))
                                                                     (FStar_Sealed.seal
                                                                     (Obj.magic
                                                                     (FStar_Range.mk_range
                                                                     "Pulse.Checker.Abs.fst"
-                                                                    (Prims.of_int (232))
+                                                                    (Prims.of_int (238))
                                                                     (Prims.of_int (10))
-                                                                    (Prims.of_int (235))
+                                                                    (Prims.of_int (241))
                                                                     (Prims.of_int (43)))))
                                                                     (Obj.magic
                                                                     (FStar_Tactics_Effect.tac_bind
@@ -1994,9 +2056,9 @@ let rec (check_abs_core :
                                                                     (Obj.magic
                                                                     (FStar_Range.mk_range
                                                                     "Pulse.Checker.Abs.fst"
-                                                                    (Prims.of_int (235))
+                                                                    (Prims.of_int (241))
                                                                     (Prims.of_int (14))
-                                                                    (Prims.of_int (235))
+                                                                    (Prims.of_int (241))
                                                                     (Prims.of_int (42)))))
                                                                     (FStar_Sealed.seal
                                                                     (Obj.magic
@@ -2011,38 +2073,33 @@ let rec (check_abs_core :
                                                                     (Pulse_Syntax_Base.C_Tot
                                                                     r)))
                                                                     (fun
-                                                                    uu___6 ->
+                                                                    uu___5 ->
                                                                     FStar_Tactics_Effect.lift_div_tac
                                                                     (fun
-                                                                    uu___7 ->
+                                                                    uu___6 ->
                                                                     Prims.strcat
                                                                     "Incorrect annotation on a function body: "
                                                                     (Prims.strcat
-                                                                    uu___6 "")))))
+                                                                    uu___5 "")))))
                                                                     (fun
-                                                                    uu___6 ->
+                                                                    uu___5 ->
                                                                     (fun
-                                                                    uu___6 ->
+                                                                    uu___5 ->
                                                                     Obj.magic
                                                                     (Pulse_Typing_Env.fail
                                                                     g
                                                                     (FStar_Pervasives_Native.Some
                                                                     (body.Pulse_Syntax_Base.range2))
-                                                                    uu___6))
-                                                                    uu___6)))
+                                                                    uu___5))
+                                                                    uu___5)))
                                                                     | 
                                                                     FStar_Pervasives_Native.Some
-                                                                    {
-                                                                    Pulse_Syntax_Base.annotated
-                                                                    = uu___5;
-                                                                    Pulse_Syntax_Base.elaborated
-                                                                    = c1;_}
-                                                                    ->
+                                                                    c1 ->
                                                                     Obj.magic
                                                                     (Obj.repr
                                                                     (FStar_Tactics_Effect.lift_div_tac
                                                                     (fun
-                                                                    uu___6 ->
+                                                                    uu___5 ->
                                                                     (c1,
                                                                     (Pulse_Syntax_Naming.open_term_nv
                                                                     (Pulse_Syntax_Base.comp_pre
@@ -2074,17 +2131,17 @@ let rec (check_abs_core :
                                                                     (Obj.magic
                                                                     (FStar_Range.mk_range
                                                                     "Pulse.Checker.Abs.fst"
-                                                                    (Prims.of_int (243))
+                                                                    (Prims.of_int (249))
                                                                     (Prims.of_int (41))
-                                                                    (Prims.of_int (243))
+                                                                    (Prims.of_int (249))
                                                                     (Prims.of_int (66)))))
                                                                     (FStar_Sealed.seal
                                                                     (Obj.magic
                                                                     (FStar_Range.mk_range
                                                                     "Pulse.Checker.Abs.fst"
-                                                                    (Prims.of_int (242))
+                                                                    (Prims.of_int (248))
                                                                     (Prims.of_int (8))
-                                                                    (Prims.of_int (273))
+                                                                    (Prims.of_int (279))
                                                                     (Prims.of_int (29)))))
                                                                     (Obj.magic
                                                                     (Pulse_Checker_Pure.check_vprop
@@ -2107,17 +2164,17 @@ let rec (check_abs_core :
                                                                     (Obj.magic
                                                                     (FStar_Range.mk_range
                                                                     "Pulse.Checker.Abs.fst"
-                                                                    (Prims.of_int (244))
+                                                                    (Prims.of_int (250))
                                                                     (Prims.of_int (16))
-                                                                    (Prims.of_int (244))
+                                                                    (Prims.of_int (250))
                                                                     (Prims.of_int (39)))))
                                                                     (FStar_Sealed.seal
                                                                     (Obj.magic
                                                                     (FStar_Range.mk_range
                                                                     "Pulse.Checker.Abs.fst"
-                                                                    (Prims.of_int (244))
+                                                                    (Prims.of_int (250))
                                                                     (Prims.of_int (42))
-                                                                    (Prims.of_int (273))
+                                                                    (Prims.of_int (279))
                                                                     (Prims.of_int (29)))))
                                                                     (FStar_Tactics_Effect.lift_div_tac
                                                                     (fun
@@ -2135,17 +2192,17 @@ let rec (check_abs_core :
                                                                     (Obj.magic
                                                                     (FStar_Range.mk_range
                                                                     "Pulse.Checker.Abs.fst"
-                                                                    (Prims.of_int (246))
+                                                                    (Prims.of_int (252))
                                                                     (Prims.of_int (8))
-                                                                    (Prims.of_int (257))
+                                                                    (Prims.of_int (263))
                                                                     (Prims.of_int (31)))))
                                                                     (FStar_Sealed.seal
                                                                     (Obj.magic
                                                                     (FStar_Range.mk_range
                                                                     "Pulse.Checker.Abs.fst"
-                                                                    (Prims.of_int (258))
+                                                                    (Prims.of_int (264))
                                                                     (Prims.of_int (8))
-                                                                    (Prims.of_int (273))
+                                                                    (Prims.of_int (279))
                                                                     (Prims.of_int (29)))))
                                                                     (match post_hint_body
                                                                     with
@@ -2167,17 +2224,17 @@ let rec (check_abs_core :
                                                                     (Obj.magic
                                                                     (FStar_Range.mk_range
                                                                     "Pulse.Checker.Abs.fst"
-                                                                    (Prims.of_int (251))
+                                                                    (Prims.of_int (257))
                                                                     (Prims.of_int (14))
-                                                                    (Prims.of_int (255))
+                                                                    (Prims.of_int (261))
                                                                     (Prims.of_int (22)))))
                                                                     (FStar_Sealed.seal
                                                                     (Obj.magic
                                                                     (FStar_Range.mk_range
                                                                     "Pulse.Checker.Abs.fst"
-                                                                    (Prims.of_int (257))
+                                                                    (Prims.of_int (263))
                                                                     (Prims.of_int (10))
-                                                                    (Prims.of_int (257))
+                                                                    (Prims.of_int (263))
                                                                     (Prims.of_int (31)))))
                                                                     (Obj.magic
                                                                     (Pulse_Checker_Base.intro_post_hint
@@ -2207,17 +2264,17 @@ let rec (check_abs_core :
                                                                     (Obj.magic
                                                                     (FStar_Range.mk_range
                                                                     "Pulse.Checker.Abs.fst"
-                                                                    (Prims.of_int (260))
+                                                                    (Prims.of_int (266))
                                                                     (Prims.of_int (19))
-                                                                    (Prims.of_int (260))
+                                                                    (Prims.of_int (266))
                                                                     (Prims.of_int (45)))))
                                                                     (FStar_Sealed.seal
                                                                     (Obj.magic
                                                                     (FStar_Range.mk_range
                                                                     "Pulse.Checker.Abs.fst"
-                                                                    (Prims.of_int (260))
+                                                                    (Prims.of_int (266))
                                                                     (Prims.of_int (48))
-                                                                    (Prims.of_int (273))
+                                                                    (Prims.of_int (279))
                                                                     (Prims.of_int (29)))))
                                                                     (FStar_Tactics_Effect.lift_div_tac
                                                                     (fun
@@ -2235,17 +2292,17 @@ let rec (check_abs_core :
                                                                     (Obj.magic
                                                                     (FStar_Range.mk_range
                                                                     "Pulse.Checker.Abs.fst"
-                                                                    (Prims.of_int (261))
+                                                                    (Prims.of_int (267))
                                                                     (Prims.of_int (15))
-                                                                    (Prims.of_int (261))
+                                                                    (Prims.of_int (267))
                                                                     (Prims.of_int (69)))))
                                                                     (FStar_Sealed.seal
                                                                     (Obj.magic
                                                                     (FStar_Range.mk_range
                                                                     "Pulse.Checker.Abs.fst"
-                                                                    (Prims.of_int (261))
+                                                                    (Prims.of_int (267))
                                                                     (Prims.of_int (73))
-                                                                    (Prims.of_int (273))
+                                                                    (Prims.of_int (279))
                                                                     (Prims.of_int (29)))))
                                                                     (Obj.magic
                                                                     (check g'
@@ -2262,17 +2319,17 @@ let rec (check_abs_core :
                                                                     (Obj.magic
                                                                     (FStar_Range.mk_range
                                                                     "Pulse.Checker.Abs.fst"
-                                                                    (Prims.of_int (263))
+                                                                    (Prims.of_int (269))
                                                                     (Prims.of_int (8))
-                                                                    (Prims.of_int (263))
+                                                                    (Prims.of_int (269))
                                                                     (Prims.of_int (61)))))
                                                                     (FStar_Sealed.seal
                                                                     (Obj.magic
                                                                     (FStar_Range.mk_range
                                                                     "Pulse.Checker.Abs.fst"
-                                                                    (Prims.of_int (261))
+                                                                    (Prims.of_int (267))
                                                                     (Prims.of_int (73))
-                                                                    (Prims.of_int (273))
+                                                                    (Prims.of_int (279))
                                                                     (Prims.of_int (29)))))
                                                                     (Obj.magic
                                                                     (Pulse_Checker_Base.apply_checker_result_k
@@ -2299,17 +2356,17 @@ let rec (check_abs_core :
                                                                     (Obj.magic
                                                                     (FStar_Range.mk_range
                                                                     "Pulse.Checker.Abs.fst"
-                                                                    (Prims.of_int (265))
+                                                                    (Prims.of_int (271))
                                                                     (Prims.of_int (6))
-                                                                    (Prims.of_int (273))
+                                                                    (Prims.of_int (279))
                                                                     (Prims.of_int (29)))))
                                                                     (FStar_Sealed.seal
                                                                     (Obj.magic
                                                                     (FStar_Range.mk_range
                                                                     "Pulse.Checker.Abs.fst"
-                                                                    (Prims.of_int (265))
+                                                                    (Prims.of_int (271))
                                                                     (Prims.of_int (6))
-                                                                    (Prims.of_int (273))
+                                                                    (Prims.of_int (279))
                                                                     (Prims.of_int (29)))))
                                                                     (FStar_Tactics_Effect.lift_div_tac
                                                                     (fun
@@ -2325,17 +2382,17 @@ let rec (check_abs_core :
                                                                     (Obj.magic
                                                                     (FStar_Range.mk_range
                                                                     "Pulse.Checker.Abs.fst"
-                                                                    (Prims.of_int (265))
+                                                                    (Prims.of_int (271))
                                                                     (Prims.of_int (6))
-                                                                    (Prims.of_int (265))
+                                                                    (Prims.of_int (271))
                                                                     (Prims.of_int (52)))))
                                                                     (FStar_Sealed.seal
                                                                     (Obj.magic
                                                                     (FStar_Range.mk_range
                                                                     "Pulse.Checker.Abs.fst"
-                                                                    (Prims.of_int (273))
+                                                                    (Prims.of_int (279))
                                                                     (Prims.of_int (6))
-                                                                    (Prims.of_int (273))
+                                                                    (Prims.of_int (279))
                                                                     (Prims.of_int (29)))))
                                                                     (Obj.magic
                                                                     (check_effect_annotation
@@ -2365,7 +2422,7 @@ let rec (check_abs_core :
                                                                     = qual;
                                                                     Pulse_Syntax_Base.ascription
                                                                     =
-                                                                    FStar_Pervasives_Native.None;
+                                                                    Pulse_Syntax_Base.empty_ascription;
                                                                     Pulse_Syntax_Base.body
                                                                     =
                                                                     (Pulse_Syntax_Naming.close_st_term
@@ -2425,13 +2482,13 @@ let (check_abs :
           (FStar_Sealed.seal
              (Obj.magic
                 (FStar_Range.mk_range "Pulse.Checker.Abs.fst"
-                   (Prims.of_int (277)) (Prims.of_int (10))
-                   (Prims.of_int (277)) (Prims.of_int (28)))))
+                   (Prims.of_int (283)) (Prims.of_int (10))
+                   (Prims.of_int (283)) (Prims.of_int (28)))))
           (FStar_Sealed.seal
              (Obj.magic
                 (FStar_Range.mk_range "Pulse.Checker.Abs.fst"
-                   (Prims.of_int (278)) (Prims.of_int (2))
-                   (Prims.of_int (278)) (Prims.of_int (26)))))
+                   (Prims.of_int (284)) (Prims.of_int (2))
+                   (Prims.of_int (284)) (Prims.of_int (26)))))
           (Obj.magic (preprocess_abs g t))
           (fun uu___ ->
              (fun t1 -> Obj.magic (check_abs_core g t1 check)) uu___)
