pulse/share/steel/examples/pulse/bug-reports/PulseLambdas.fst
@@ -23,15 +23,15 @@ fn swap (#a:Type0) (x y:ref a) (#vx #vy:erased a)
 ```
 
 
-let swap_fun a = x:ref a -> y:ref a -> #vx:erased a -> #vy:erased a -> stt unit
+let swap_fun = #a:Type0 -> x:ref a -> y:ref a -> #vx:erased a -> #vy:erased a -> stt unit
     (requires pts_to x vx ** pts_to y vy)
     (ensures fun _ -> pts_to x vy ** pts_to y vx)
 
 
 ```pulse
-fn test_top_level_lambda (#a:Type0)
-  : swap_fun a
-  = (x y:_) (#vx #vy:_)
+fn test_top_level_lambda (_:unit) // should allow nullary "lambdas"
+  : swap_fun 
+  = (#a:Type0) (x y #_vx #_vy:_)
     {
       let vx = !x;
       let vy = !y;
@@ -41,23 +41,26 @@ fn test_top_level_lambda (#a:Type0)
 ```
 
 
-let t = test_top_level_lambda
-// [@@expect_failure]
-// ```pulse
-// fn test_inner_lambda (#a:Type0)
-//                      (x y:ref int)
-// requires pts_to x 'vx ** pts_to y 'vy
-// ensures  pts_to x 'vy ** pts_to y 'vx
-// {
-//   fn write_helper (#a:Type) (x:ref a) (n:a)
-//     requires pts_to x 'vx
-//     ensures  pts_to x n
-//   {
-//     x := n;
-//   };
-//   let vx = !x;
-//   let vy = !y;
-//   write_helper x vy;
-//   write_helper y vy;
-// } 
-// ```
+
+
+let w = test_top_level_lambda
+[@@expect_failure]
+```pulse
+fn test_inner_lambda (#a:Type0)
+                     (x y:ref int)
+requires pts_to x 'vx ** pts_to y 'vy
+ensures  pts_to x 'vy ** pts_to y 'vx
+{
+  ghost
+  fn write_helper (#a:Type) (x:ref a) (n:a)
+    requires pts_to x 'vx
+    ensures  pts_to x n
+  {
+    x := n;
+  };
+  let vx = !x;
+  let vy = !y;
+  write_helper x vy;
+  write_helper y vy;
+} 
+```
