pulse/lib/steel/pulse/Pulse.Syntax.Base.fsti
@@ -178,9 +178,10 @@ type proof_hint_type =
 noeq
 type comp_ascription = {
   annotated:option comp;
-  elaborated:comp
+  elaborated:option comp
 }
-  
+let empty_ascription = { annotated=None; elaborated=None }  
+
 (* terms with STT types *)
 [@@ no_auto_projectors]
 noeq
@@ -193,7 +194,7 @@ type st_term' =
   | Tm_Abs {
       b:binder;
       q:option qualifier;
-      ascription: option comp_ascription;
+      ascription: comp_ascription;
       body:st_term;
     }
   | Tm_STApp {
